src/Init/Data/Iterators/Lemmas/Consumers/Monadic/Collect.lean
@@ -44,11 +44,11 @@ theorem IterM.DefaultConsumers.toArrayMapped.go.aux₂ [Monad n] [LawfulMonad n]
 theorem IterM.DefaultConsumers.toArrayMapped_eq_match_step [Monad n] [LawfulMonad n]
     [Iterator α m β] [Finite α m] :
     IterM.DefaultConsumers.toArrayMapped lift f it (m := m) = letI : MonadLift m n := ⟨lift (δ := _)⟩; (do
-      match ← it.step with
-      | .yield it' out _ =>
+      match (← it.step).val with
+      | .yield it' out =>
         return #[← f out] ++ (← IterM.DefaultConsumers.toArrayMapped lift f it' (m := m))
-      | .skip it' _ => IterM.DefaultConsumers.toArrayMapped lift f it' (m := m)
-      | .done _ => return #[]) := by
+      | .skip it' => IterM.DefaultConsumers.toArrayMapped lift f it' (m := m)
+      | .done => return #[]) := by
   rw [IterM.DefaultConsumers.toArrayMapped, IterM.DefaultConsumers.toArrayMapped.go]
   apply bind_congr
   intro step
@@ -57,10 +57,10 @@ theorem IterM.DefaultConsumers.toArrayMapped_eq_match_step [Monad n] [LawfulMona
 theorem IterM.toArray_eq_match_step [Monad m] [LawfulMonad m] [Iterator α m β] [Finite α m]
     [IteratorCollect α m m] [LawfulIteratorCollect α m m] :
     it.toArray = (do
-      match ← it.step with
-      | .yield it' out _ => return #[out] ++ (← it'.toArray)
-      | .skip it' _ => it'.toArray
-      | .done _ => return #[]) := by
+      match (← it.step).val with
+      | .yield it' out => return #[out] ++ (← it'.toArray)
+      | .skip it' => it'.toArray
+      | .done => return #[]) := by
   simp only [IterM.toArray, LawfulIteratorCollect.toArrayMapped_eq]
   rw [IterM.DefaultConsumers.toArrayMapped_eq_match_step]
   simp [bind_pure_comp, pure_bind, toArray]
@@ -78,10 +78,10 @@ theorem IterM.toArray_toList [Monad m] [LawfulMonad m] [Iterator α m β] [Finit
 theorem IterM.toList_eq_match_step [Monad m] [LawfulMonad m] [Iterator α m β] [Finite α m]
     [IteratorCollect α m m] [LawfulIteratorCollect α m m] {it : IterM (α := α) m β} :
     it.toList = (do
-      match ← it.step with
-      | .yield it' out _ => return out :: (← it'.toList)
-      | .skip it' _ => it'.toList
-      | .done _ => return []) := by
+      match (← it.step).val with
+      | .yield it' out => return out :: (← it'.toList)
+      | .skip it' => it'.toList
+      | .done => return []) := by
   simp [← IterM.toList_toArray]
   rw [IterM.toArray_eq_match_step, map_eq_pure_bind, bind_assoc]
   apply bind_congr
@@ -111,10 +111,10 @@ theorem IterM.toListRev.go.aux₂ [Monad m] [LawfulMonad m] [Iterator α m β] [
 theorem IterM.toListRev_eq_match_step [Monad m] [LawfulMonad m] [Iterator α m β] [Finite α m]
     {it : IterM (α := α) m β} :
     it.toListRev = (do
-      match ← it.step with
-      | .yield it' out _ => return (← it'.toListRev) ++ [out]
-      | .skip it' _ => it'.toListRev
-      | .done _ => return []) := by
+      match (← it.step).val with
+      | .yield it' out => return (← it'.toListRev) ++ [out]
+      | .skip it' => it'.toListRev
+      | .done => return []) := by
   simp [IterM.toListRev]
   rw [toListRev.go]
   apply bind_congr
@@ -131,7 +131,11 @@ theorem IterM.reverse_toListRev [Monad m] [LawfulMonad m] [Iterator α m β] [Fi
   rw [toListRev_eq_match_step, toList_eq_match_step, map_eq_pure_bind, bind_assoc]
   apply bind_congr
   intro step
-  split <;> simp (discharger := assumption) [ihy, ihs]
+  split
+  all_goals
+    rename_i heq
+    have := heq ▸ step.property
+    simp (discharger := assumption) [ihy, ihs]
 
 theorem IterM.toListRev_eq [Monad m] [LawfulMonad m] [Iterator α m β] [Finite α m]
     [IteratorCollect α m m] [LawfulIteratorCollect α m m]
